SystemF2Effect; doing liveS_deallocate lemma
Ignore-this: 4415a4b2eee91133ffa7c8718baa64f2

darcs-hash:20130406122543-08f32-ac0c9f2988367bfa08662d45a8b51a5fb421e0fc

devel/Iron/SystemF2Effect/Store/Bind.v
@@ -37,3 +37,17 @@ Definition regionOfStBind (b : stbind)
 Hint Unfold regionOfStBind.
 
 
+(* Deallocate all store bindings in the given region by setting
+   them to StDead. The dead bindings hold their locations in the
+   store, but they no longer contain any value. *)
+Fixpoint deallocate (p1 : nat) (ss : store) : store
+ := match ss with
+    |  nil                   => nil
+    |  StValue p2 v :: ss' 
+    => if beq_nat p1 p2
+           then StDead  p2   :: deallocate p1 ss'
+           else StValue p2 v :: deallocate p1 ss'
+   
+    |  StDead p2 :: ss' 
+    => StDead p2 :: deallocate p1 ss'
+    end.
